smc-next/UCCore.ec
@@ -1,0 +1,509 @@
+(* UCCore.eca *)
+
+prover quorum=2 ["Alt-Ergo" "Z3"].
+
+(* Core UC Definitions and Lemmas *)
+
+require import AllCore List FSet ListPO Encoding.
+
+(* real protocols and ideal functionalities (collectively,
+   "functionalities") have hierarchical addresses
+
+   if a functionality has address alpha, it is also responsible for all
+   sub-functionalities with addresses beta >= alpha (in the prefix
+   partial ordering of ListPO)
+
+   adversaries are also modeled as functionalities - but with no
+   subaddresses/sub-functionalties; simulators are functionalities
+   parameterized by adversaries *)
+
+type addr = int list.
+
+(* ports - pairs of functionality addresses and port indices
+
+   a functionality's ports are used/interpreted however the
+   functionality chooses, but typically they are divided into
+   different parties
+
+   adversaries can handle multiple port indices, and each simulator
+   has a single port index *)
+
+type port = addr * int.
+
+(* messages have modes:
+
+     * direct - supplying functionality inputs, consuming their
+         outputs
+
+     * adversarial - communication between functionalties and
+         adversaries/simulators, communication between different
+         adversaries/simulators, and communication between
+         environments and adversaries/simulators *)
+
+type mode = [
+    Dir  (* direct *)
+  | Adv  (* adversarial *)
+].
+
+lemma not_dir (mod : mode) :
+  mod <> Dir <=> mod = Adv.
+proof. by case mod. qed.
+
+lemma not_adv (mod : mode) :
+  mod <> Adv <=> mod = Dir.
+proof. by case mod. qed.
+
+(* begin theory parameters *)
+
+type univ.  (* universe of values *)
+
+(* universe encoding/decoding operators - more can be added by
+   other theories *)
+
+(* univ encoding: port * int * univ *)
+
+clone EPDP as EPDP_Univ_PortIntUniv with
+  type orig <- port * int * univ,
+  type enc  <- univ.
+
+(* end theory parameters *)
+
+(* a message has the form (mod, pt1, pt2, u), for a mode mod, a
+   destination port pt1, a source port pt2, and a universe
+   value u *)
+
+type msg = mode * port * port * univ.
+
+(* guard an optional message using predicate *)
+
+op opt_msg_guard :
+     (mode -> addr -> int -> addr -> int -> univ -> bool) ->
+     msg option -> msg option =
+     fun f : mode -> addr -> int -> addr -> int -> univ -> bool =>
+     fun m_opt : msg option =>
+       match m_opt with
+         None   => None
+       | Some m =>
+           if f m.`1 m.`2.`1 m.`2.`2 m.`3.`1 m.`3.`2 m.`4
+           then m_opt
+           else None
+       end.
+
+(* module type used for real protocols and ideal functionalities
+   (collectively, "functionalities"), as well as adversaries and
+   simulators *)
+
+pred func_init_pre (self adv : addr) = inc self adv.
+
+module type FUNC = {
+  (* initialize functionality (or adversary), telling it its address
+     (self) and the address of its adversary (adv)
+
+     in the case of the adversary, the second argument will be [], the
+     root address of the environment (so the adversary's "adversary" is
+     the environment)
+
+     precondition for ordinary (non-adversary) functionalties:
+     func_init_pre self adv *)
+
+  proc init(self adv : addr) : unit
+
+  (* respond to an incoming message, producing an optional
+     outgoing message (None means error)
+
+     messages to a functionality should have addresses that are >=
+     self (in the case of an adversary, = self)
+
+     if Some m' is returned, then the destination address of m' should
+     not be >= self, and the source address of m' should be >= self
+     (in the case of an adversary, the source address should be =
+     self) *)
+
+  proc invoke(m : msg) : msg option
+}.
+
+(* module type of interfaces (to environment): consists of
+   a functionality part and an adversary part *)
+
+pred inter_init_pre (func adv : addr) = inc func adv.
+
+module type INTER = {
+  (* initialize interface, telling it:
+
+       * the address (func) of its functionality part;
+
+       * the address (adv) of its adversary part;
+
+       * an incoming message guard (in_guard)
+
+     the interface will initialize its functionality and adversary
+     parts; when calling the adversary part's init function, the
+     second argument will be [], the root address of the environment
+
+     precondition:
+
+       inter_init_pre func adv *)
+
+  proc init(func adv : addr, in_guard : int fset) : unit
+
+  (* respond to an incoming message, producing an optional
+     outgoing message (None means error)
+
+     messages whose destination addresses aren't either >= the
+     interface's functionality part's address, func, or *equal* to the
+     interface's adversary part's addresss, adv, should result in None
+     being returned
+
+     all incoming messages with mode Dir must be addressed to the
+     interface's functionality part (else None is returned); all
+     incoming messages with mode Adv must be addressed to the
+     interface's adversary part (else None is returned)
+
+     if the interface's functionality part returns a message with
+     destination address >= func, or if the interface's adversary part
+     returns a message with destination address >= adv, then
+     None should be returned
+
+     if the interface's functionality part returns a message with
+     source address not >= func, or if the interface's adversary part
+     returns a message with source address <> adv, then None should be
+     returned
+
+     all outgoing messages with mode Dir come from the interface's
+     functionality part; all outgoing messages with mode Adv come from
+     the interface's adversary part
+
+     the standard (Adv mode) channel between the environment and the
+     interface's adversary part consists of messages between port
+     ([], 0) (in the environment) and port (adv, 0) (in the
+     interface's adversary part)
+
+     the environment may communicate with other port indices of the
+     interface's adversary part, except that such a communication will
+     result in an error if its destination port isn't of the form
+     (adv, n) for some n in in_guard
+
+     if the interface's functionality part sends a message to the
+     interface's adversary port (destination address must be = adv),
+     this message must have mode Adv, and it may not have destination
+     port (adv, 0)
+
+     if the interface's adversary port sends a message to the
+     interface's functionality part, this message must have mode
+     Adv *)
+
+  proc invoke(m : msg) : msg option
+}.
+
+(* module type of environments, parameterized by interfaces *)
+
+pred env_init_pre (func adv : addr) = inter_init_pre func adv.
+
+module type ENV (Inter : INTER) = {
+  (* start environment, and let it interact with Inter (only via
+     Inter.invoke, not via Inter.init), eventually returning a boolean
+     judgment
+
+     we have:
+
+       * func is the address of interface's functionality part
+
+       * adv is the address of interface's adversary part
+
+     the standard (Adv mode) channel between the environment and the
+     interface's adversary part consists of messages between port
+     ([], 0) (in the environment) and port (adv, 0) (in the
+     interface's adversary part)
+
+     the environment may communicate with other ports of the
+     interface's adversary part, except that such a communication will
+     result in an error if its destination port isn't of the form
+     (adv, n) for some n in in_guard
+
+     precondition : env_pre func adv *)
+
+  proc main(func adv : addr, in_guard : int fset) : bool {Inter.invoke}
+}.
+
+(* carry out experiment in which the environment is allowed to
+   interact with, and issue a final boolean judgment about, an
+   interface, which is first initialized *)
+
+pred exper_pre (func adv : addr) = inter_init_pre func adv.
+
+lemma exper_pre_ext1 (func adv ext : addr) :
+  exper_pre func adv => exper_pre (func ++ ext) adv.
+proof.
+rewrite /exper_pre /inter_init_pre.
+move => |> inc_fun_adv.
+by apply inc_ext1.
+qed.
+
+module Exper (Inter : INTER, Env : ENV) = {
+  module E = Env(Inter)
+
+  (* arguments to main:
+
+       * func is address of interface's functionality part
+
+       * adv is the address of the interface's adversary part
+
+       * in_guard is the incoming message guard used by the interface
+         and supplied to the environment
+
+     precondition:
+
+       exper_pre func adv *)
+
+  proc main(func adv : addr, in_guard : int fset) : bool = {
+    var b : bool;
+    Inter.init(func, adv, in_guard);
+    b <@ E.main(func, adv, in_guard);
+    return b;
+  }    
+}.
+
+(* make interface out of functionality and adversary parts *)
+
+abstract theory MakeInterface.
+
+module MI (Func : FUNC, Adv : FUNC) : INTER = {
+  var func, adv : addr
+  var in_guard : int fset
+
+  proc init(func_ adv_ : addr, in_guard_ : int fset) : unit = {
+    func <- func_; adv <- adv_; in_guard <- in_guard_;
+    Func.init(func, adv);
+    Adv.init(adv, []);
+  }
+
+  proc loop(m : msg) : msg option = {
+    var r : msg option <- None;
+    var not_done : bool <- true;
+
+    (* loop invariant in terms of m:
+
+         not_done =>
+         func <= m.`2.`1 \/
+         m.`1 = Adv /\ m.`2.`1 = adv *)
+
+    while (not_done) {
+      if (func <= m.`2.`1) {
+        r <@ Func.invoke(m);
+        if (r = None) {
+          not_done <- false;
+        }
+        else {
+          m <- oget r;  (* next iteration, if any, will use m *)
+          if (func <= m.`2.`1 \/ ! func <= m.`3.`1) {
+            r <- None; not_done <- false;
+          }
+          elif (m.`1 = Dir) {
+            not_done <- false;
+            if (adv <= m.`2.`1) {
+              r <- None;
+            }
+          }
+          elif (m.`2.`1 <> adv \/ m.`2.`2 = 0) {
+            r <- None; not_done <- false;
+          }
+        }          
+      }
+      else {  (* m.`1 = Adv /\ m.`2.`1 = adv *)
+        r <@ Adv.invoke(m);
+        if (r = None) {
+          not_done <- false;
+        }
+        else {
+          m <- oget r;  (* next iteration, if any, will use m *)
+          if (m.`1 = Dir \/ adv <= m.`2.`1 \/ ! adv <> m.`3.`1) {
+            r <- None; not_done <- false;
+          }
+          elif (! func <= m.`2.`1) {
+            not_done <- false;
+          }
+        }
+      }      
+    }
+    return r;
+  }
+
+  proc invoke(m : msg) : msg option = {
+    var r : msg option;
+    if ((m.`1 = Dir /\ func <= m.`2.`1 \/
+         m.`1 = Adv /\ m.`2.`1 = adv /\
+         (m.`2.`2 = 0 \/ m.`2.`2 \in in_guard)) /\
+        ! func <= m.`3.`1 /\ ! adv <= m.`3.`1) {
+      r <@ loop(m);
+    }
+    else {
+      r <- None;
+    }
+    return r;
+  }
+}.
+
+end MakeInterface.
+
+(* dummy adversary (DA) - completely controlled by environment *)
+
+abstract theory DummyAdversary.
+
+(* message from port ([], 0) of environment to port (dfe_da, 0) of
+   dummy adversary, instructing dummy adversary to send message (Adv,
+   dfe_pt, (dfe_da, dfe_n), dfe_u); dfa_n should not be 0, and
+   dfe_pt should not be [] or be >= address of DA *)
+
+type da_from_env =
+  {dfe_da : addr;   (* address of dummy adversary *)
+   (* data: *)
+   dfe_pt : port;   (* destination port of message to be sent by DA *)
+   dfe_n  : int;    (* source port index of message to be sent by DA *)
+   dfe_u  : univ}.  (* value of message to be sent by DA *)
+
+op da_from_env (x : da_from_env) : msg =
+     (Adv, (x.`dfe_da, 0), ([], 0),
+      EPDP_Univ_PortIntUniv.enc (x.`dfe_pt, x.`dfe_n, x.`dfe_u)).
+
+op dec_da_from_env (m : msg) : da_from_env option =
+     let (mod, pt1, pt2, v) = m
+     in (mod = Dir \/ pt1.`2 <> 0 \/ pt2 <> ([], 0) \/
+         ! EPDP_Univ_PortIntUniv.valid v) ?
+        None :
+        let (pt, n, u) = oget (EPDP_Univ_PortIntUniv.dec v)
+        in Some {|dfe_da = pt1.`1; dfe_pt = pt; dfe_n = n; dfe_u = u|}.
+
+lemma epdp_da_from_env : epdp da_from_env dec_da_from_env.
+proof.
+apply epdp_intro.
+move => x.
+rewrite /da_from_env /dec_da_from_env /= EPDP_Univ_PortIntUniv.valid_enc
+        /= EPDP_Univ_PortIntUniv.enc_dec oget_some /#.
+move => [mod pt1 pt2 u] v.
+rewrite /da_from_env /dec_da_from_env /=.
+case (mod = Dir \/ pt1.`2 <> 0 \/ pt2 <> ([], 0) \/
+      ! (EPDP_Univ_PortIntUniv.valid u)) => //.
+rewrite !negb_or /= not_dir => [#] -> pt1_2 -> val_u.
+have [] t : exists (t : port * int * univ), EPDP_Univ_PortIntUniv.dec u = Some t.
+  exists (oget (EPDP_Univ_PortIntUniv.dec u)); by rewrite -some_oget.
+move => /EPDP_Univ_PortIntUniv.dec_enc <-.
+rewrite EPDP_Univ_PortIntUniv.enc_dec oget_some /#.
+qed.
+
+lemma dest_valid_da_from_env (m : msg) :
+  dec2valid dec_da_from_env m =>
+  m.`2.`1 = (oget (dec_da_from_env m)).`dfe_da /\ m.`2.`2 = 0.
+proof.
+move => val_m.
+have [] x : exists (x : da_from_env), dec_da_from_env m = Some x.
+  exists (oget (dec_da_from_env m)); by rewrite -some_oget.
+case x => x1 x2 x3 x4.
+move => /(epdp_dec_enc _ _ _ _ epdp_da_from_env) <-.
+by rewrite (epdp_enc_dec _ _ _ epdp_da_from_env).
+qed.
+
+lemma source_valid_da_from_env (m : msg) :
+  dec2valid dec_da_from_env m => m.`3 = ([], 0).
+proof.
+move => val_m.
+have [] x : exists (x : da_from_env), dec_da_from_env m = Some x.
+  exists (oget (dec_da_from_env m)); by rewrite -some_oget.
+case x => x1 x2 x3 x4.
+move => /(epdp_dec_enc _ _ _ _ epdp_da_from_env) => <- //.
+qed.
+
+(* message from port (da, 0) of dummy adversary to port ([], 0) of
+   environment, telling environment that dummy adversary received
+   message (Adv, (da, n), pt, u) *)
+
+type da_to_env =
+  {dte_da : addr;   (* address of dummy adversary *)
+   (* data: *)
+   dte_pt : port;   (* source port of message sent to DA *)
+   dte_n  : int;    (* destination port index of message sent to DA *)
+   dte_u  : univ}.  (* value of message sent to DA *)
+
+op da_to_env (x : da_to_env) : msg =
+     (Adv, ([], 0), (x.`dte_da, 0), 
+      EPDP_Univ_PortIntUniv.enc(x.`dte_pt, x.`dte_n, x.`dte_u)).
+
+op dec_da_to_env (m : msg) : da_to_env option =
+     let (mod, pt1, pt2, v) = m
+     in (mod = Dir \/ pt1 <> ([], 0) \/ pt2.`2 <> 0 \/
+         ! EPDP_Univ_PortIntUniv.valid v) ?
+        None :
+        let (pt, n, u) = oget (EPDP_Univ_PortIntUniv.dec v)
+        in Some {|dte_da = pt2.`1; dte_pt = pt; dte_n = n; dte_u = u|}.
+
+lemma epdp_da_to_env : epdp da_to_env dec_da_to_env.
+proof.
+apply epdp_intro.
+move => x.
+rewrite /da_to_env /dec_da_to_env /= EPDP_Univ_PortIntUniv.valid_enc
+        /= EPDP_Univ_PortIntUniv.enc_dec oget_some /#.
+move => [mod pt1 pt2 u] v.
+rewrite /da_to_env /dec_da_to_env /=.
+case (mod = Dir \/ pt1 <> ([], 0) \/ pt2.`2 <> 0 \/
+      ! (EPDP_Univ_PortIntUniv.valid u)) => //.
+rewrite !negb_or /= not_dir => [#] -> -> pt2_2 val_u.
+have [] t : exists (t : port * int * univ), EPDP_Univ_PortIntUniv.dec u = Some t.
+  exists (oget (EPDP_Univ_PortIntUniv.dec u)); by rewrite -some_oget.
+move => /EPDP_Univ_PortIntUniv.dec_enc <-.
+rewrite EPDP_Univ_PortIntUniv.enc_dec oget_some /#.
+qed.
+
+lemma dest_valid_da_to_env (m : msg) :
+  dec2valid dec_da_to_env m =>
+  m.`3.`1 = (oget (dec_da_to_env m)).`dte_da /\ m.`3.`2 = 0.
+proof.
+move => val_m.
+have [] x : exists (x : da_to_env), dec_da_to_env m = Some x.
+  exists (oget (dec_da_to_env m)); by rewrite -some_oget.
+case x => x1 x2 x3 x4.
+move => /(epdp_dec_enc _ _ _ _ epdp_da_to_env) <-.
+by rewrite (epdp_enc_dec _ _ _ epdp_da_to_env).
+qed.
+
+lemma source_valid_da_to_env (m : msg) :
+  dec2valid dec_da_to_env m => m.`2 = ([], 0).
+proof.
+move => val_m.
+have [] x : exists (x : da_to_env), dec_da_to_env m = Some x.
+  exists (oget (dec_da_to_env m)); by rewrite -some_oget.
+case x => x1 x2 x3 x4.
+move => /(epdp_dec_enc _ _ _ _ epdp_da_to_env) => <- //.
+qed.
+
+module DummyAdv : FUNC = {
+  var self, env : addr
+
+  proc init(self_ env_ : addr) = {
+    self <- self_; env <- env_;
+  }
+
+  proc invoke(m : msg) : msg option = {
+    var r : msg option <- None;
+
+    match (dec_da_from_env m) with
+      Some x => {  (* message from ([], 0); m.`2.`2 = 0 *)
+        if (x.`dfe_da = self /\ x.`dfe_n <> 0 /\
+            x.`dfe_pt.`1 <> [] /\ !self <= x.`dfe_pt.`1 ) {
+          r <- Some (Adv, x.`dfe_pt, (self, x.`dfe_n), x.`dfe_u);
+        }
+      }
+    | None   => {
+        (* message from functionality; we should have
+           m.`1 = Adv /\ m.`2.`1 = self /\ m.`2.`2 <> 0 /\
+           ! self <= m.`3.`1 *)
+        r <-
+          Some
+          (da_to_env
+           {|dte_da = self; dte_pt = m.`3; dte_n = m.`2.`2;
+             dte_u = m.`4|});
+      }
+    end;
+    return r;
+  }
+}.
+
+end DummyAdversary.
